cellio/CtxA.v
@@ -3,7 +3,7 @@ Require Import MainHeader CellioHeader CtxHeader.
 
 Set Implicit Arguments.
 
-Module CtxHdr.
+(* Module CtxHdr.
 
   Definition mn := "Ctx".
     
@@ -13,15 +13,14 @@ Module CtxHdr.
   Definition foo := fn "foo".
   Definition input := fn "input".
 
-End CtxHdr.
-
+End CtxHdr. *)
 
 Module CtxAS.
 Section CtxAS.
   Context `{Σ: GRA}.
 
-  Definition sp: alist string fspec :=
-    Seal.sealing CRIS [(CtxHdr.foo, fspec_trivial); (CtxHdr.input, fspec_trivial)].
+  Definition sp: spl_type :=
+    Seal.sealing CRIS [(Some CtxHdr.foo, Some fspec_trivial); (Some CtxHdr.input, Some fspec_trivial)].
   
   Lemma sp_nodup: List.NoDup (List.map fst sp).
   Proof.
