cellio/MainI.v
@@ -6,7 +6,7 @@ Set Implicit Arguments.
 Module MainI. Section MainI.
   Context `{Σ: GRA}.
 
-  Definition scopes := [MainHdr.mn].
+  Definition scopes := ["Main"].
 
   Definition main: Any.t -> itree hmodE Any.t :=
     λ _,
@@ -16,16 +16,16 @@ Module MainI. Section MainI.
       trigger (@IO _ unit "Print" x);;;
       Ret tt↑.
   
-  Definition fnsems :=
-    [(MainHdr.main, (wmask_all, scopes, main))].
+  Definition fnsems : alist (option string) (fnsem_type (option fspec * fbody)) :=
+    [(MainHdr.main, (false, wmask_all, scopes, (None, main)))].
 
-  Program Definition Mod: PMod.t := {|
-    PMod.scopes := scopes;
-    PMod.fnsems := fnsems;
-    PMod.initial_st := [];
+  Program Definition Mod: SMod.t := {|
+    SMod.scopes := scopes;
+    SMod.fnsems := fnsems;
+    SMod.initial_st := [];
   |}.
   Solve All Obligations with prove_scope.
   Next Obligation. prove_nodup. Qed.
   
-  Definition t := Seal.sealing CRIS (PMod.to_hmod Mod).
+  Definition t := Seal.sealing CRIS (SMod.to_hmod sp_none Mod).
 End MainI. End MainI.
