cellio/MainIAproof.v
@@ -5,7 +5,7 @@ Set Implicit Arguments.
 
 Module MainIA. Section MainIA.
   Import CellioA.
-  Context `{_sinvG: !sinvG Γ Σ α β τ _I _S}.
+  Context `{!crisG Γ Σ α β τ _I _S}.
   Context `{_cellioG: !cellioG}.
 
   Definition Ist: nat -> alist key Any.t -> alist key Any.t -> iProp Σ :=
@@ -19,21 +19,27 @@ Module MainIA. Section MainIA.
   Local Definition IstFull := (IstProd (IstSB MainA.(HMod.scopes) Ist) IstEq).
 
   Lemma simF_main:
-    HSim.sim_fun open MainA (MainI.t ★ CellioA) IstFull MainHdr.main.
+    HSim.sim_fun open MainA (MainI.t ★ CellioA) MainA.InitCond IstFull MainHdr.main.
   Proof using CtxInSp.
     init_simF.
     
     (* Take cell(0) *)
     steps_l; iDestruct "ASM" as "[ASM %]"; subst.
 
-    inline_r.
+    steps_r. inline_r.
     (* Give cell(0) *)
     steps_r. forces_r. iSplitL ""; eauto.
     forces_r. iSplitL "ASM"; eauto.
 
     (* Call Input() simultaneously *)
     steps_r. forces_l. iSplitL "GRT"; eauto.
-    call "IST"; eauto.
+    call "IST". 
+    {
+      iDestruct "IST" as "[[-> [-> ->]] IC]".
+      repeat iExists []. iSplit; eauto;
+      repeat unfold_hmod; ss;
+      repeat (iSplit; eauto); iPureIntro; prove_scope.
+    }
     steps_l. forces_r. iSplitL "ASM"; eauto.
     steps_r. hss.
 
@@ -68,8 +74,7 @@ Module MainIA. Section MainIA.
     HSim.t open MainA (MainI.t ★ CellioA) MainA.InitCond IstFull.
   Proof using CtxInSp.
     init_sim.
-    - iIntros "_". repeat iExists []. iSplit; eauto.
-      repeat (iSplit; eauto); iPureIntro; prove_scope.
+    - exfalso. revert H0. rewrite /MainI.t /CellioA. unseal CRIS; ss.
     - eapply simF_main; eauto.
   Qed.
 End MainIA. End MainIA.
